## T1

$$
\begin{aligned}
  \delta S 
  &=  - \delta \int {dt{e^{ - \phi {\text{(f)}}}}\sqrt {1 - {{f'}^2}} }  \cr 
   &= \int {dt\frac{{\delta \phi }}{{\delta f}}{e^{ - \phi {\text{(f)}}}}\sqrt {1 - {{f'}^2}} \delta f}  + \int {dt{e^{ - \phi {\text{(f)}}}}\frac{{f'}}{{\sqrt {1 - {{f'}^2}} }}\delta f'}  \cr 
   &= \int {dt\frac{{\delta \phi }}{{\delta f}}{e^{ - \phi {\text{(f)}}}}\sqrt {1 - {{f'}^2}} \delta f}  - \int {dt\frac{d}{{dt}}\left( {{e^{ - \phi {\text{(f)}}}}\frac{{f'}}{{\sqrt {1 - {{f'}^2}} }}} \right)\delta f}  \cr 
   &= \int {dt\frac{{\delta \phi }}{{\delta f}}{e^{ - \phi {\text{(f)}}}}\sqrt {1 - {{f'}^2}} \delta f}  - \int {dt{e^{ - \phi {\text{(f)}}}}\frac{d}{{dt}}\left( {\frac{{f'}}{{\sqrt {1 - {{f'}^2}} }}} \right)\delta f}  \cr 
   &= \int {dt\frac{{\delta \phi }}{{\delta f}}{e^{ - \phi {\text{(f)}}}}\sqrt {1 - {{f'}^2}} \delta f}  - \int {dt{e^{ - \phi {\text{(f)}}}}\frac{{f''\left( {1 - {{f'}^2}} \right) + {{f'}^2}}}{{{{\left( {1 - {{f'}^2}} \right)}^{\frac{3}{2}}}}}\delta f}  
   \end{aligned}
$$



进而得到
$$
\frac{{\delta \phi }}{{\delta f}}{e^{ - \phi {\text{(f)}}}}\sqrt {1 - {{f'}^2}}  - {e^{ - \phi {\text{(f)}}}}\frac{{f''\left( {1 - {{f'}^2}} \right) + {{f'}^2}}}{{{{\left( {1 - {{f'}^2}} \right)}^{\frac{3}{2}}}}} =0
$$

## T2

###1

$$
\begin{aligned}
\delta S 
&= \delta \int {dt\left( {{{f'}^2} + {f^2}f'' + f{{f'}^2}f''} \right)}  \cr 
&= \int {dt\left( {2f'\delta f' + 2ff''\delta f + {f^2}\delta f'' + {{f'}^2}f''\delta f + 2ff'f''\delta f' + f{{f'}^2}\delta f''} \right)}  \cr 
&= \int {dt\left( { - 2f'' + 4ff'' + 2{{f'}^2} + {{f'}^2}f''+ 3{{f'}^2}f''} \right)\delta f}  \cr 
&= \int {dt\left( { - 2f'' + 4ff'' + 2{{f'}^2} + 4{{f'}^2}f'' } \right)\delta f}  
\end{aligned}
$$

### 2

$$
\begin{aligned}
\tilde{L}&=f'^2 - 2ff'^2 - \frac{1}{3}f'^4\\
F&=f^2f'+\frac{1}{3}ff'^3
\end{aligned}
$$

### 3

$$
\eqalign{
  & \delta \tilde S  \cr 
  &  = \delta \int {dt({{f'}^2} - 2f{{f'}^2} - \frac{1}{3}{{f'}^4})}   \cr 
  &  = \int {dt(2f'\delta f' - 2{{f'}^2}\delta f - 4ff'\delta f' - \frac{4}{3}{{f'}^3}\delta f')}   \cr 
  &  = \int {dt( - 2f'' - 2{{f'}^2} + 4ff'' + 4{{f'}^2} + 4f''{{f'}^2})\delta f}   \cr 
  &  = \int {dt( - 2f'' + 2{{f'}^2} + 4ff'' + 4f''{{f'}^2})\delta f}  \cr} 
$$



## T3

略

## T4

