```math
\begin{align}
L_i
&=r_j p_k\epsilon_{ijk}\\
\frac{\part L_i}{\part r_\alpha}
&=\epsilon_{ijk}p_k\delta_{\alpha j}-\epsilon_{ijk}p_j\delta_{\alpha k}\\
&=\epsilon_{i\alpha k}p_k-\epsilon_{ij\alpha}p_j\\
\frac{\part L_i}{\part p_\alpha}
&=\epsilon_{ij\alpha}r_j-\epsilon_{i\alpha k}r_k\\
\end{align}
```

```math
\frac{\part L_1}{\part r_2}
&=2p_3\\
```

```math
\frac{\part L_1}{\part p_2}
&=-2r_3\\
```

```math
\frac{\part L_3}{\part p_2}
&=2r_1\\
```

```math
\frac{\part L_3}{\part r_2}
&=-2p_1\\
```

