### 4.

åˆ†ä¸¤éƒ¨åˆ†è®¡ç®—ï¼ˆçº¯è®¡ç®—ï¼Œæ²¡ä»€ä¹ˆå¥‡æ€ªç©æ„ï¼‰

> PSï¼Œæˆ‘ä»¬ç›´æ¥å‡å®šå¾®åˆ†å¯æ¢åºäº†ğŸ˜¡å®ƒè‚¯å®šå¯æ¢åºğŸ˜¡

$$
\eqalign{
  & \frac{{\partial {A^\mu }}}{{\partial {x^\nu }}}  \cr 
  &  = \frac{{\partial {A^\mu }}}{{\partial {{x'}^\alpha }}}\frac{{\partial {{x'}^\alpha }}}{{\partial {x^\nu }}}  \cr 
  &  = \frac{{\partial \left( {\frac{{\partial {x^\mu }}}{{\partial {{x'}^\beta }}}{{A'}^\beta }} \right)}}{{\partial {{x'}^\alpha }}}\frac{{\partial {{x'}^\alpha }}}{{\partial {x^\nu }}}  \cr 
  &  = \frac{{\partial {{x'}^\alpha }}}{{\partial {x^\nu }}}\left( {\frac{{{\partial ^2}{x^\mu }}}{{\partial {{x'}^\alpha }\partial {{x'}^\beta }}}{{A'}^\beta } + \frac{{\partial {x^\mu }}}{{\partial {{x'}^\beta }}}{{A'}^\beta }_{,\alpha }} \right)  \cr 
  &  = \frac{{\partial {{x'}^\alpha }}}{{\partial {x^\nu }}}\frac{{\partial {x^\mu }}}{{\partial {{x'}^\beta }}}{{A'}^\beta }_{,\alpha } + \frac{{\partial {{x'}^\alpha }}}{{\partial {x^\nu }}}\frac{{{\partial ^2}{x^\mu }}}{{\partial {{x'}^\alpha }\partial {{x'}^\beta }}}{{A'}^\beta }  \cr 
  &  = \frac{{\partial {{x'}^\alpha }}}{{\partial {x^\nu }}}\frac{{\partial {x^\mu }}}{{\partial {{x'}^\beta }}}{{A'}^\beta }_{,\alpha } + \frac{{{\partial ^2}{x^\mu }}}{{\partial {x^\nu }\partial {{x'}^\beta }}}{{A'}^\beta }  \cr 
  &  = \frac{{\partial {{x'}^\alpha }}}{{\partial {x^\nu }}}\frac{{\partial {x^\mu }}}{{\partial {{x'}^\beta }}}{{A'}^\beta }_{,\alpha } \cr}
$$

ç¬¬äºŒéƒ¨åˆ†
$$
\eqalign{
  & \Gamma _{\lambda \nu }^\mu {A^\lambda }  \cr 
  &  = \left( {{\Gamma '}_{\alpha \sigma }^\rho \frac{{\partial {{x'}^\alpha }}}{{\partial {x^\lambda }}}\frac{{\partial {{x'}^\sigma }}}{{\partial {x^\nu }}}\frac{{\partial {x^\mu }}}{{\partial {{x'}^\rho }}} + \frac{{{\partial ^2}{{x'}^\rho }}}{{\partial {x^\lambda }\partial {x^\nu }}}\frac{{\partial {x^\mu }}}{{\partial {{x'}^\rho }}}} \right){A^\lambda }  \cr 
  &  = \left( {{\Gamma '}_{\alpha \sigma }^\rho \frac{{\partial {{x'}^\alpha }}}{{\partial {x^\lambda }}}\frac{{\partial {{x'}^\sigma }}}{{\partial {x^\nu }}}\frac{{\partial {x^\mu }}}{{\partial {{x'}^\rho }}} + \frac{{{\partial ^2}{{x'}^\rho }}}{{\partial {x^\lambda }\partial {x^\nu }}}\frac{{\partial {x^\mu }}}{{\partial {{x'}^\rho }}}} \right)\left( {\frac{{\partial {x^\lambda }}}{{\partial {{x'}^\beta }}}{{A'}^\beta }} \right)  \cr 
  &  = {\Gamma '}_{\alpha \sigma }^\rho \frac{{\partial {{x'}^\alpha }}}{{\partial {x^\lambda }}}\frac{{\partial {{x'}^\sigma }}}{{\partial {x^\nu }}}\frac{{\partial {x^\mu }}}{{\partial {{x'}^\rho }}}\frac{{\partial {x^\lambda }}}{{\partial {{x'}^\beta }}}{{A'}^\beta } + \frac{{{\partial ^2}{{x'}^\rho }}}{{\partial {{x'}^\beta }\partial {x^\nu }}}\frac{{\partial {x^\mu }}}{{\partial {{x'}^\rho }}}{{A'}^\beta }  \cr 
  &  = \frac{{\partial {{x'}^\alpha }}}{{\partial {x^\nu }}}\frac{{\partial {x^\mu }}}{{\partial {{x'}^\beta }}}{\Gamma '}_{\sigma \alpha }^\beta {{A'}^\sigma } \cr} 
$$
